cogent/examples/wa_connect/Generated_CorresSetup.thy
@@ -40,6 +40,18 @@ end
 class cogent_C_heap = cogent_C_val +
   fixes is_valid    :: "lifted_globals \<Rightarrow> 'a ptr \<Rightarrow> bool"
   fixes heap        :: "lifted_globals \<Rightarrow> 'a ptr \<Rightarrow> 'a"
+
+instantiation WordArray_u32_C :: cogent_C_val
+begin
+definition type_rel_WordArray_u32_C_def: 
+  "type_rel typ (_ :: WordArray_u32_C itself) \<equiv> typ = RCon ''WordArray'' [RPrim (Num U32)]"
+definition val_rel_WordArray_u32_C_def:
+  "val_rel uv (x :: WordArray_u32_C) \<equiv> (\<exists>len arr. uv = UAbstract (WAU32 len arr) \<and> 
+                                                  len = (SCAST(32 signed \<rightarrow> 32)(len_C x)) \<and>
+                                                  arr = ptr_val (values_C x))"
+instance ..
+end
+
 local_setup \<open> local_setup_val_rel_type_rel_put_them_in_buckets "main_pp_inferred.c" \<close>
 local_setup \<open> local_setup_instantiate_cogent_C_heaps_store_them_in_buckets "main_pp_inferred.c" \<close>
 locale Generated = "main_pp_inferred" + update_sem_init
@@ -104,6 +116,7 @@ lemmas val_rel_simps[ValRelSimp] =
   val_rel_unit_t_C_def
   val_rel_bool_t_C_def
   val_rel_fun_tag
+  val_rel_WordArray_u32_C_def
 
 lemmas type_rel_simps[TypeRelSimp] =
   type_rel_word
@@ -111,6 +124,7 @@ lemmas type_rel_simps[TypeRelSimp] =
   type_rel_unit_def
   type_rel_unit_t_C_def
   type_rel_bool_t_C_def
+  type_rel_WordArray_u32_C_def
 
 (* Generating the specialised take and put lemmas *)
 
